refactoring

Network_Security_Policy_Verification/NetworkModel_ENF.thy
@@ -347,4 +347,297 @@ section {* instance helper *}
 
 
 
+
+
+(*ENF_sr*)
+
+
+section {* edges normal form ENF with sender and receiver names *}
+  definition (in NetworkModel_withOffendingFlows) eval_model_all_edges_normal_form_sr :: "('a \<Rightarrow> 'v \<Rightarrow> 'a \<Rightarrow> 'v \<Rightarrow> bool) \<Rightarrow> bool" where
+    "eval_model_all_edges_normal_form_sr P \<equiv> \<forall> G nP. eval_model G nP = (\<forall> (s, r)\<in> edges G. P (nP s) s (nP r) r)"
+  
+
+  lemma (in NetworkModel_withOffendingFlows) ENFsr_monotonicity_eval_model_mono: "\<lbrakk> eval_model_all_edges_normal_form_sr P \<rbrakk> \<Longrightarrow>
+    eval_model_mono"
+    apply(simp add: eval_model_all_edges_normal_form_sr_def eval_model_mono_def)
+    by blast
+
+section {* offending flows:*}
+  
+  theorem (in NetworkModel_withOffendingFlows) ENFsr_offending_set:
+    assumes ENFsr: "eval_model_all_edges_normal_form_sr P"
+    shows "set_offending_flows G nP = (if eval_model G nP then
+      {}
+     else 
+      { {(s,r). (s, r) \<in> edges G \<and> \<not> P (nP s) s (nP r) r} })" (is "?A = ?B")
+  proof(cases "eval_model G nP")
+  case True thus "?A = ?B" 
+    by(simp add: set_offending_flows_def is_offending_flows_min_set_def is_offending_flows_def)
+  next
+  case False
+   from ENFsr have ENFsr_offending_imp_not_P: "\<And> F s r. F \<in> set_offending_flows G nP \<Longrightarrow> (s, r) \<in> F  \<Longrightarrow> \<not> P (nP s) s (nP r) r"
+     unfolding eval_model_all_edges_normal_form_sr_def
+     apply(simp add: set_offending_flows_def is_offending_flows_def is_offending_flows_min_set_def graph_ops)
+     apply clarify
+     by fastforce
+   from ENFsr have  ENFsr_offending_set_P_representation: 
+    "\<And> F. F \<in> set_offending_flows G nP  \<Longrightarrow> F = {(s,r). (s, r) \<in> edges G \<and> \<not> P (nP s) s (nP r) r}"
+      apply -
+      apply rule
+       apply rule
+       apply clarify
+       apply(rename_tac a b)
+       apply rule
+        apply(auto simp add:set_offending_flows_def)[1]
+       apply(simp add: ENFsr_offending_imp_not_P)
+      unfolding eval_model_all_edges_normal_form_sr_def
+      apply(simp add:set_offending_flows_def is_offending_flows_def is_offending_flows_min_set_def graph_ops)
+      apply clarify
+      apply(rename_tac a b a1 b1)
+      apply(blast)
+    done
+  
+
+    from ENFsr False have ENFsr_offending_flows_exist: "set_offending_flows G nP \<noteq> {}"
+      apply(simp add: set_offending_flows_def is_offending_flows_min_set_def is_offending_flows_def eval_model_all_edges_normal_form_sr_def
+            delete_edges_def add_edge_def)
+      apply(clarify)
+      apply(rename_tac s r)
+      apply(rule_tac x="{(s,r). (s,r) \<in> (edges G) \<and> \<not>P (nP s) s (nP r) r}" in exI)
+      apply(simp)
+      by blast
+
+    from ENFsr have ENFsr_offenindg_not_empty_imp_ENF_offending_subseteq_rhs:
+      "set_offending_flows G nP \<noteq> {}  \<Longrightarrow>
+      { {(s,r). (s, r) \<in> edges G \<and> \<not> P (nP s) s (nP r) r} } \<subseteq> set_offending_flows G nP"
+      apply -
+      apply rule
+      using ENFsr_offending_set_P_representation
+      by blast
+
+    from ENFsr have ENFsr_offending_subseteq_lhs:
+      "(set_offending_flows G nP) \<subseteq> { {(s,r). (s, r) \<in> edges G \<and> \<not> P (nP s) s (nP r) r} }"
+      apply -
+      apply rule
+      by(simp add: ENFsr_offending_set_P_representation)
+
+    from False ENFsr_offenindg_not_empty_imp_ENF_offending_subseteq_rhs[OF ENFsr_offending_flows_exist] ENFsr_offending_subseteq_lhs show "?A = ?B"
+      by force
+  qed
+  
+
+
+
+(*ENFnrSR*)
+
+section {* edges normal form not refl ENFnrSR *}
+  definition (in NetworkModel_withOffendingFlows) eval_model_all_edges_normal_form_not_refl_SR :: "('a \<Rightarrow> 'v \<Rightarrow> 'a \<Rightarrow> 'v \<Rightarrow> bool) \<Rightarrow> bool" where
+    "eval_model_all_edges_normal_form_not_refl_SR P \<equiv> 
+    \<forall> G nP. eval_model G nP = (\<forall> (s, r) \<in> edges G. s \<noteq> r \<longrightarrow> P (nP s) s (nP r) r)"
+
+
+
+  text{* we derive everything from the ENFnrSR form *}
+  lemma (in NetworkModel_withOffendingFlows) ENFnrSR_to_ENFsr: 
+    "eval_model_all_edges_normal_form_not_refl_SR P \<Longrightarrow> eval_model_all_edges_normal_form_sr (\<lambda> p1 v1 p2 v2. v1 \<noteq> v2 \<longrightarrow> P p1 v1 p2 v2)"
+    by(simp add: eval_model_all_edges_normal_form_sr_def eval_model_all_edges_normal_form_not_refl_SR_def)
+    
+
+
+section {*offending flows*}
+   theorem (in NetworkModel_withOffendingFlows) ENFnrSR_offending_set:
+    "\<lbrakk> eval_model_all_edges_normal_form_not_refl_SR P \<rbrakk> \<Longrightarrow>
+    set_offending_flows G nP = (if eval_model G nP then
+      {}
+     else 
+      { {(e1,e2). (e1, e2) \<in> edges G \<and> e1 \<noteq> e2 \<and> \<not> P (nP e1) e1 (nP e2) e2} })"
+    by(auto dest: ENFnrSR_to_ENFsr simp: ENFsr_offending_set)
+
+
+section {* Instance helper*}
+
+  (* fsts version *)
+  lemma (in NetworkModel_withOffendingFlows)  ENFnrSR_fsts_weakrefl_instance:
+    fixes "default_node_properties" :: "'a" ("\<bottom>")
+    assumes a_enf: "eval_model_all_edges_normal_form_not_refl_SR P"
+    and   a_weakrefl: "\<forall> s r. P \<bottom> s \<bottom> r"
+    and   a_botdefault: "\<forall> s r. (nP r) \<noteq> \<bottom> \<longrightarrow> \<not> P (nP s) s (nP r) r \<longrightarrow> \<not> P \<bottom> s (nP r) r"
+    and   a_alltobot: "\<forall> s r. P (nP s) s \<bottom> r"
+    and   a_offending: "f \<in> set_offending_flows G nP"
+    and   a_i_fsts: "i \<in> fst` f"
+    shows
+          "\<not> eval_model G (nP(i := \<bottom>))"
+  proof -
+    from a_offending have a_not_eval: "\<not> eval_model G nP" by (metis ex_in_conv validmodel_imp_no_offending)
+    from valid_without_offending_flows[OF a_offending] have a_offending_rm: "eval_model (delete_edges G f) nP" .
+    from a_enf have a_enf': "\<And> G nP. eval_model G nP  = (\<forall> (e1, e2)\<in> (edges G). e1 \<noteq> e2 \<longrightarrow> P (nP e1) e1 (nP e2) e2)" 
+      using eval_model_all_edges_normal_form_not_refl_SR_def by simp
+  
+    from ENFnrSR_offending_set[OF a_enf] a_not_eval a_offending have a_f_3_in_f: "\<And> e1 e2. (e1, e2)\<in>f \<Longrightarrow> \<not> P (nP e1) e1 (nP e2) e2" by(simp)
+    from ENFnrSR_offending_set[OF a_enf] a_not_eval a_offending have a_f_3_neq: "\<And> e1 e2. (e1, e2)\<in>f \<Longrightarrow> e1 \<noteq> e2" by simp
+  
+    let ?nP' = "(nP(i := \<bottom>))"
+
+    from ENFnrSR_offending_set[OF a_enf] a_not_eval a_offending a_i_fsts
+      obtain e1 e2 where e1e2cond: "(e1, e2) \<in> f \<and> e1 = i" by fastforce
+
+    from conjunct1[OF e1e2cond] a_offending have "(e1, e2) \<in> edges G"
+      by (metis (lifting, no_types) NetworkModel_withOffendingFlows.set_offending_flows_def mem_Collect_eq set_rev_mp)
+  
+    from conjunct1[OF e1e2cond] a_f_3_in_f have e1e2notP: "\<not> P (nP e1) e1 (nP e2) e2" by simp
+    from e1e2notP a_weakrefl have e1ore2neqbot: "(nP e1) \<noteq> \<bottom> \<or> (nP e2) \<noteq> \<bottom>" by fastforce
+    from e1e2notP a_alltobot have "(nP e2) \<noteq> \<bottom>" by fastforce
+    from this e1e2notP a_botdefault have "\<not> P \<bottom> e1 (nP e2) e2" by simp
+    from this e1e2notP have e1e2subgoal1: "\<not> P (?nP' e1) e1 (nP e2) e2" by auto
+
+    from a_f_3_neq e1e2cond have "e2 \<noteq> e1" by blast
+  
+    from e1e2subgoal1 have "e1 \<noteq> e2 \<Longrightarrow> \<not> P (?nP' e1) e1 (?nP' e2) e2"
+      apply simp
+      apply(rule conjI)
+       apply blast
+      apply(insert e1e2cond)
+      by simp
+    from this `e2 \<noteq> e1` have "\<not> P (?nP' e1) e1 (?nP' e2) e2" by simp
+  
+    from this `e2 \<noteq> e1` ENFnrSR_offending_set[OF a_enf] a_offending `(e1, e2) \<in> edges G` have 
+      "\<exists> (e1, e2)\<in>(edges G). e2 \<noteq> e1 \<and> \<not> P (?nP' e1) e1 (?nP' e2) e2" by blast
+    hence "\<not> (\<forall> (e1, e2)\<in>(edges G). e2 \<noteq> e1 \<longrightarrow> P ((nP(i := \<bottom>)) e1) e1 ((nP(i := \<bottom>)) e2) e2)" by fast
+    from this a_enf' show "\<not> eval_model G (nP(i := \<bottom>))" by fast
+  qed
+
+
+
+  (* snds version *)
+  lemma (in NetworkModel_withOffendingFlows)  ENFnrSR_snds_weakrefl_instance:
+    fixes "default_node_properties" :: "'a" ("\<bottom>")
+    assumes a_enf: "eval_model_all_edges_normal_form_not_refl_SR P"
+    and   a_weakrefl: "\<forall> s r. P \<bottom> s \<bottom> r"
+    and   a_botdefault: "\<forall> s r. (nP s) \<noteq> \<bottom> \<longrightarrow> \<not> P (nP s) s (nP r) r \<longrightarrow> \<not> P (nP s) s \<bottom> r"
+    and   a_bottoall: "\<forall> s r. P \<bottom> s (nP r) r"
+    and   a_offending: "f \<in> set_offending_flows G nP"
+    and   a_i_snds: "i \<in> snd` f"
+    shows
+          "\<not> eval_model G (nP(i := \<bottom>))"
+  proof -
+    from a_offending have a_not_eval: "\<not> eval_model G nP" by (metis equals0D validmodel_imp_no_offending)
+    from valid_without_offending_flows[OF a_offending] have a_offending_rm: "eval_model (delete_edges G f) nP" .
+    from a_enf have a_enf': "\<And> G nP. eval_model G nP  = (\<forall> (e1, e2)\<in>(edges G). e1 \<noteq> e2 \<longrightarrow> P (nP e1) e1 (nP e2) e2)" 
+      using eval_model_all_edges_normal_form_not_refl_SR_def by simp
+  
+    from ENFnrSR_offending_set[OF a_enf] a_not_eval a_offending have a_f_3_in_f: "\<And> s r. (s, r)\<in>f \<Longrightarrow> \<not> P (nP s) s (nP r) r" by simp
+    from ENFnrSR_offending_set[OF a_enf] a_not_eval a_offending have a_f_3_neq: "\<And> s r. (s, r)\<in>f \<Longrightarrow> s \<noteq> r" by simp
+  
+    let ?nP' = "(nP(i := \<bottom>))"
+
+    from ENFnrSR_offending_set[OF a_enf] a_not_eval a_offending a_i_snds
+      obtain e1 e2 where e1e2cond: "(e1, e2)\<in>f \<and> e2 = i" by fastforce
+
+    from conjunct1[OF e1e2cond] a_offending have "(e1, e2) \<in> edges G"
+      by (metis (lifting, no_types) NetworkModel_withOffendingFlows.set_offending_flows_def mem_Collect_eq set_rev_mp)
+  
+    from conjunct1[OF e1e2cond] a_f_3_in_f have e1e2notP: "\<not> P (nP e1) e1 (nP e2) e2" by simp
+    from e1e2notP a_weakrefl have e1ore2neqbot: "(nP e1) \<noteq> \<bottom> \<or> (nP e2) \<noteq> \<bottom>" by fastforce
+    from e1e2notP a_bottoall have x1: "(nP e1) \<noteq> \<bottom>" by fastforce
+    from this e1e2notP a_botdefault have x2: "\<not> P (nP e1) e1 \<bottom> e2" by fast
+    from this e1e2notP have e1e2subgoal1: "\<not> P (nP e1) e1 (?nP' e2) e2" by auto
+
+    from a_f_3_neq e1e2cond have "e2 \<noteq> e1" by blast
+  
+    from e1e2subgoal1 have "e1 \<noteq> e2 \<Longrightarrow> \<not> P (?nP' e1) e1 (?nP' e2) e2" by(simp add: e1e2cond)
+  
+    from this `e2 \<noteq> e1` ENFnrSR_offending_set[OF a_enf] a_offending `(e1, e2) \<in> edges G` have 
+      "\<exists> (e1, e2)\<in>(edges G). e2 \<noteq> e1 \<and> \<not> P (?nP' e1) e1 (?nP' e2) e2" by fastforce
+    hence "\<not> (\<forall> (e1, e2)\<in>(edges G). e2 \<noteq> e1 \<longrightarrow> P ((nP(i := \<bottom>)) e1) e1 ((nP(i := \<bottom>)) e2) e2)" by fast
+    from this a_enf' show "\<not> eval_model G (nP(i := \<bottom>))" by fast
+  qed
+
+
+
+
+(*ENFnr*)
+
+
+
+section {* edges normal form not refl ENFnr *}
+  definition (in NetworkModel_withOffendingFlows) eval_model_all_edges_normal_form_not_refl :: "('a \<Rightarrow> 'a \<Rightarrow> bool) \<Rightarrow> bool" where
+    "eval_model_all_edges_normal_form_not_refl P \<equiv> \<forall> G nP. eval_model G nP = (\<forall> (e1, e2) \<in> edges G. e1 \<noteq> e2 \<longrightarrow> P (nP e1) (nP e2))"
+  
+
+  text{* we derive everything from the ENFnrSR form *}
+  lemma (in NetworkModel_withOffendingFlows) ENFnr_to_ENFnrSR: 
+    "eval_model_all_edges_normal_form_not_refl P \<Longrightarrow> eval_model_all_edges_normal_form_not_refl_SR (\<lambda> v1 _ v2 _. P v1 v2)"
+    by(simp add: eval_model_all_edges_normal_form_not_refl_def eval_model_all_edges_normal_form_not_refl_SR_def)
+
+  (*most of results are now implied from previous lemma*)
+
+section {*offending flows*}
+   theorem (in NetworkModel_withOffendingFlows) ENFnr_offending_set:
+    "\<lbrakk> eval_model_all_edges_normal_form_not_refl P \<rbrakk> \<Longrightarrow>
+    set_offending_flows G nP = (if eval_model G nP then
+      {}
+     else 
+      { {(e1,e2). (e1, e2) \<in> edges G \<and> e1 \<noteq> e2 \<and> \<not> P (nP e1) (nP e2)} })"
+    apply(drule ENFnr_to_ENFnrSR)
+    by(drule(1) ENFnrSR_offending_set)
+
+
+section {* Instance helper*}
+  (* fsts version *)
+  lemma (in NetworkModel_withOffendingFlows)  ENFnr_fsts_weakrefl_instance:
+    fixes "default_node_properties" :: "'a" ("\<bottom>")
+    assumes a_enf: "eval_model_all_edges_normal_form_not_refl P"
+    and   a_botdefault: "\<forall> e1 e2. e2 \<noteq> \<bottom> \<longrightarrow> \<not> P e1 e2 \<longrightarrow> \<not> P \<bottom> e2"
+    and   a_alltobot: "\<forall> e1. P e1 \<bottom>"
+    and   a_offending: "f \<in> set_offending_flows G nP"
+    and   a_i_fsts: "i \<in> fst` f"
+    shows
+          "\<not> eval_model G (nP(i := \<bottom>))"
+  proof -
+    from assms show ?thesis
+    apply -
+    apply(drule ENFnr_to_ENFnrSR)
+    apply(drule ENFnrSR_fsts_weakrefl_instance)
+         by auto
+  qed
+  
+  (* snds version *)
+  lemma (in NetworkModel_withOffendingFlows)  ENFnr_snds_weakrefl_instance:
+    fixes "default_node_properties" :: "'a" ("\<bottom>")
+    assumes a_enf: "eval_model_all_edges_normal_form_not_refl P"
+    and   a_botdefault: "\<forall> e1 e2. \<not> P e1 e2 \<longrightarrow> \<not> P e1 \<bottom>"
+    and   a_bottoall: "\<forall> e2. P \<bottom> e2"
+    and   a_offending: "f \<in> set_offending_flows G nP"
+    and   a_i_snds: "i \<in> snd` f"
+    shows
+          "\<not> eval_model G (nP(i := \<bottom>))"
+  proof -
+    from assms show ?thesis
+    apply -
+    apply(drule ENFnr_to_ENFnrSR)
+    apply(drule ENFnrSR_snds_weakrefl_instance)
+         by auto
+  qed
+ 
+
+
+
+  (* snds version DRAFT*)
+  lemma (in NetworkModel_withOffendingFlows)  ENF_weakrefl_instance_FALSE:
+    fixes "default_node_properties" :: "'a" ("\<bottom>")
+    assumes a_validG: "valid_graph G"
+    and   a_not_eval: "\<not> eval_model G nP"
+    and   a_enf: "eval_model_all_edges_normal_form P"
+    and   a_weakrefl: "P \<bottom> \<bottom>"
+    and   a_botisolated: "\<And> e2. e2 \<noteq> \<bottom> \<Longrightarrow> \<not> P \<bottom> e2"
+    and   a_botdefault: "\<And> e1 e2. e1 \<noteq> \<bottom> \<Longrightarrow> \<not> P e1 e2 \<Longrightarrow> \<not> P e1 \<bottom>"
+    and   a_offending: "f \<in> set_offending_flows G nP"
+    and   a_offending_rm: "eval_model (delete_edges G f) nP"
+    and   a_i_fsts: "i \<in> snd` f"
+    and   a_not_eval_upd: "\<not> eval_model G (nP(i := \<bottom>))"
+    shows "False"
+oops
+
+
+
 end
